revise KmsArn? resource part
make sure resource length >=2. and add witness* after subset type KmsArn

KmsArnIdentifier.dfy
@@ -5,24 +5,39 @@ predicate ArnString?(s: string)
 // MUST start with string arn
 type ArnString = s:string | ArnString?(s) witness "arn"
 
+
+
+// The partition MUST be a non-empty
 predicate PartitionString?(s:string)
 {
     s != ""
 }
-
-// The partition MUST be a non-empty
 type PartitionString = s:string | PartitionString?(s) witness *
+
+
 
 // The service MUST be the string kms
 predicate ServiceString?(s:string)
+{
+    s == "kms"
+}
 
-type ServiceString = s | s =="kms" witness *
+type ServiceString = s | ServiceString?(s) witness *
 
 // The region MUST be a non-empty string
-type RegionString = s:string | |s| != 0 witness *
+predicate RegionString?(s:string)
+{
+    |s|!=0
+}
+type RegionString = s:string | RegionString?(s) witness *
 
 //The account MUST be a non-empty string
-type AccountString = s:string | |s| != 0 witness *
+predicate AccountString?(s:string)
+{
+    |s|!=0
+
+}
+type AccountString = s:string | AccountString?(s) witness *
 
 
 // The resource section MUST be non-empty and MUST be split by a single / any additional / are included in the resource id
@@ -30,7 +45,12 @@ type AccountString = s:string | |s| != 0 witness *
 // The resource id MUST be a non-empty string 
 // this seq<string> length is 2, x[0] is key, x[1] is ID.
 
-type KmsResourceSeqStr = x:seq<string> | |x| == 2 && (x[0]=="alias" || x[0] == "key") && |x[1]| != 0
+predicate KmsResourceSeqStr?(x:seq<string>)
+{
+    |x| == 2 && (x[0]=="alias" || x[0] == "key") && |x[1]| != 0
+}
+
+type KmsResourceSeqStr = x:seq<string> | KmsResourceSeqStr?(x) witness *
 
 datatype ARN = ARN(
     arnLiteral: string,
@@ -43,10 +63,12 @@ datatype ARN = ARN(
 
 
 
-type KmsArn = a: ARN | KmsArn?(a)
+type KmsArn = a: ARN | KmsArn?(a) witness *
 
 
 predicate KmsArn?(a:ARN)
+
+
 {
     if
         // MUST start with string arn
@@ -65,6 +87,7 @@ predicate KmsArn?(a:ARN)
         && |a.region| !=0
 
         // then it leads to resource type to be key or alias, and both id cannot be empty
+        &&  |a.resource|>=2
         &&  (
             (&& a.resource[0] == "key"
             && |a.resource[1]|!=0 ) 
@@ -80,7 +103,6 @@ method test()
 {
     assert ARN("arn","aws","kms","us-east-1","2222222222222",["key","testid"]).ARN?;
 
-
-    assert KmsArn?(ARN("arn","aws","kms","us-east-1","2222222222222",["key","testid"])) == true;
+    assert KmsArn?(ARN("arn","aws","kms","us-east-1","2222222222222",["alias","testid"])) == true;
 
 }
